src/Cps_Trans.v
@@ -1,72 +1,31 @@
 Require Import Core_Infrastructure Source_Definitions Target_Definitions
                Source_Properties Target_Properties.
 
+(* for applications where the type argument is irrelevant *)
 Definition dummy_type := t_typ_bool.
 
-Lemma s_type_arrow_inv_l : forall s1 s2,
- s_type (s_typ_arrow s1 s2) -> s_type s1.
-Proof. inversion 1. assumption. Qed.
+Fixpoint cps_type_trans (s:typ) :=
+  match s with
+    | s_typ_bool => t_typ_bool
+    | s_typ_arrow s1 s2 =>
+      t_typ_arrow (t_typ_pair (cps_type_trans s1)
+                              (t_typ_arrow (cps_type_trans s2) (t_typ_bvar 1)))
+                  (t_typ_bvar 0)
+    | _ => typ_bad
+  end.
 
-Lemma s_type_arrow_inv_r : forall s1 s2,
- s_type (s_typ_arrow s1 s2) -> s_type s2.
-Proof. inversion 1. assumption. Qed.
+Notation "( s +)" := (cps_type_trans s) (at level 0).
 
-Definition cps_type_trans (s:typ) (wf : s_type s) : typ.
- induction s; try solve [elimtype False; inversion wf].
- (* bool+ = bool *)
- exact t_typ_bool.
- (* (s1->s2)+ = forall a, s1+ X ((s2+ -> a) -> a) *)
- exact (t_typ_arrow (t_typ_pair (IHs1 (s_type_arrow_inv_l s1 s2 wf))
-                                (t_typ_arrow (IHs2 (s_type_arrow_inv_r s1 s2 wf))
-                                             (t_typ_bvar 1)))
-                    (t_typ_bvar 0)).
-Defined.
-
-Lemma cps_type_trans_bool : forall wf,
-  cps_type_trans s_typ_bool wf = t_typ_bool.
-Proof. auto. Qed.
-
-Lemma cps_type_trans_arrow : forall s1 s2 wf,
-  cps_type_trans (s_typ_arrow s1 s2) wf = 
-  t_typ_arrow (t_typ_pair (cps_type_trans s1 (s_type_arrow_inv_l s1 s2 wf))
-                          (t_typ_arrow
-                            (cps_type_trans s2 (s_type_arrow_inv_r s1 s2 wf))
-                            (t_typ_bvar 1)))
-              (t_typ_bvar 0).
-Proof. intros. simpl. f_equal. Qed.
-
-Lemma cps_type_trans_produces_t_type : forall s wf_s,
-  t_type (cps_type_trans s wf_s).
+Lemma cps_type_trans_preserves_well_formed_types : forall s,
+  s_type s -> t_type (s+).
 Proof.
-  induction s; intros; auto; try solve [elimtype False; inversion wf_s].
-  rewrite cps_type_trans_arrow.
-  apply_fresh t_type_arrow as X. simpl.
-  apply t_type_pair.
-  rewrite open_tt_rec_t_type; apply IHs1.
-  apply_fresh t_type_arrow as Y.
-  rewrite open_tt_rec_t_type; rewrite open_tt_rec_t_type; apply IHs2.
-  apply t_type_var. apply t_type_var.
+  induction 1; auto.
+  simpl. apply_fresh t_type_arrow as X; simpl; auto.
+  apply t_type_pair; rewrite* open_tt_rec_t_type.
+  apply_fresh t_type_arrow as Y; rewrite* open_tt_rec_t_type.
 Qed.
 
-Extraction cps_type_trans. (* BAM *)
+Definition cps_type_trans_computation (s : typ) :=
+  t_typ_arrow (t_typ_arrow (s+) (t_typ_bvar 1)) (t_typ_bvar 0).
 
-Definition cps_type_trans_computation (s : typ) (wf : s_type s) :=
-  t_typ_arrow (t_typ_arrow (cps_type_trans s wf) (t_typ_bvar 1))
-              (t_typ_bvar 0).
-
-Eval simpl in cps_type_trans (s_typ_arrow s_typ_bool s_typ_bool).
-
-Fixpoint cps_term_trans (G:env_term) (e:trm) (s:typ)
-  (s_der : s_typing G e s) : trm :=
-match e with
-| s_trm_true => t_trm_abs (t_typ_arrow (cps_type_trans s)
-                                       (t_typ_bvar 0)) (* \[a](k:bool->a). *)
-                          (t_trm_app (t_trm_bvar 0)    (*        k true    *)
-                                     dummy_type
-                                     t_trm_true)
-| _ => t_trm_false
-end.
-
-Eval simpl in
-  cps_term_trans empty s_trm_true s_typ_bool
-                 (s_typing_true empty (LibWfenv.wfenv_empty s_type)).
+Notation "( s %)" := (cps_type_trans_computation s) (at level 0).
